cleanup: unify ERC721 addressed contract (#1325)

Contracts/ERC721/Contract.lean
@@ -1,30 +1,30 @@
-import Contracts.MacroContracts.ERC721Addressed
+import Contracts.MacroContracts.ERC721
 
 namespace Contracts.ERC721
 
-abbrev owner := Contracts.MacroContracts.ERC721Addressed.owner
-abbrev totalSupply := Contracts.MacroContracts.ERC721Addressed.totalSupply
-abbrev nextTokenId := Contracts.MacroContracts.ERC721Addressed.nextTokenId
-abbrev balances := Contracts.MacroContracts.ERC721Addressed.balances
-abbrev owners := Contracts.MacroContracts.ERC721Addressed.owners
-abbrev tokenApprovals := Contracts.MacroContracts.ERC721Addressed.tokenApprovals
-abbrev operatorApprovals := Contracts.MacroContracts.ERC721Addressed.operatorApprovals
+abbrev owner := Contracts.MacroContracts.ERC721.owner
+abbrev totalSupply := Contracts.MacroContracts.ERC721.totalSupply
+abbrev nextTokenId := Contracts.MacroContracts.ERC721.nextTokenId
+abbrev balances := Contracts.MacroContracts.ERC721.balances
+abbrev owners := Contracts.MacroContracts.ERC721.owners
+abbrev tokenApprovals := Contracts.MacroContracts.ERC721.tokenApprovals
+abbrev operatorApprovals := Contracts.MacroContracts.ERC721.operatorApprovals
 
-abbrev addressToWord := Contracts.MacroContracts.ERC721Addressed.addressToWord
-abbrev wordToAddress := Contracts.MacroContracts.ERC721Addressed.wordToAddress
-abbrev boolToWord := Contracts.MacroContracts.ERC721Addressed.boolToWord
+abbrev addressToWord := Contracts.MacroContracts.ERC721.addressToWord
+abbrev wordToAddress := Contracts.MacroContracts.ERC721.wordToAddress
+abbrev boolToWord := Contracts.MacroContracts.ERC721.boolToWord
 
-abbrev isOwner := Contracts.MacroContracts.ERC721Addressed.isOwner
-abbrev onlyOwner := Contracts.MacroContracts.ERC721Addressed.onlyOwner
+abbrev isOwner := Contracts.MacroContracts.ERC721.isOwner
+abbrev onlyOwner := Contracts.MacroContracts.ERC721.onlyOwner
 
-abbrev «constructor» := Contracts.MacroContracts.ERC721Addressed.constructor
-abbrev balanceOf := Contracts.MacroContracts.ERC721Addressed.balanceOf
-abbrev ownerOf := Contracts.MacroContracts.ERC721Addressed.ownerOf
-abbrev getApproved := Contracts.MacroContracts.ERC721Addressed.getApproved
-abbrev isApprovedForAll := Contracts.MacroContracts.ERC721Addressed.isApprovedForAll
-abbrev approve := Contracts.MacroContracts.ERC721Addressed.approve
-abbrev setApprovalForAll := Contracts.MacroContracts.ERC721Addressed.setApprovalForAll
-abbrev mint := Contracts.MacroContracts.ERC721Addressed.mint
-abbrev transferFrom := Contracts.MacroContracts.ERC721Addressed.transferFrom
+abbrev «constructor» := Contracts.MacroContracts.ERC721.«constructor»
+abbrev balanceOf := Contracts.MacroContracts.ERC721.balanceOf
+abbrev ownerOf := Contracts.MacroContracts.ERC721.ownerOf
+abbrev getApproved := Contracts.MacroContracts.ERC721.getApproved
+abbrev isApprovedForAll := Contracts.MacroContracts.ERC721.isApprovedForAll
+abbrev approve := Contracts.MacroContracts.ERC721.approve
+abbrev setApprovalForAll := Contracts.MacroContracts.ERC721.setApprovalForAll
+abbrev mint := Contracts.MacroContracts.ERC721.mint
+abbrev transferFrom := Contracts.MacroContracts.ERC721.transferFrom
 
 end Contracts.ERC721
